Toward SR

proof/CCPD.alaChen/Inversion.v
@@ -3,11 +3,14 @@ Require Import Reduction.
 Require Import Conv.
 Require Import LiftSubst.
 Require Import Env.
+Require Import Reduction.
 Require Import CCPD.Types.
 Require Import CCPD.Thinning.
 Require Import CCPD.Substitution.
 Require Import CCPD.Coercion.
+Require Import CCPD.GenerationNotKind.
 Require Import CCPD.Generation.
+Require Import CCPD.GenerationCoerce.
 Require Import CCPD.UnicityOfSorting.
 
 Set Implicit Arguments.
@@ -17,101 +20,238 @@ Implicit Type s : sort.
 Implicit Types A B M N T t u v : term.
 Implicit Types e f g : env.
 
-
-
-  Definition inv_type (P : Prop) e t T s : Prop :=
+Definition inv_type (P : Prop) e t T : Prop :=
     match t with
     | Srt prop => T = (Srt kind) -> P
     | Srt set => T = (Srt kind) -> P
     | Srt kind => True
     | Ref n => forall x : term, item _ x e n -> 
-       e |- T : Srt s -> e |- T >> (lift (S n) x) : s -> P
+      forall s, e |- T >> (lift (S n) x) : s -> P
     | Abs A M =>
         forall s1 (U : term),
         typ e A (Srt s1) ->
-        typ (A :: e) M U -> coerce e T (Prod A U) s -> P
+        typ (A :: e) M U -> 
+        forall s, coerce e T (Prod A U) s -> P
     | App u v =>
         forall Ur V : term,
         typ e v V -> typ e u (Prod V Ur) -> 
-        typ e T (Srt s) ->
-        coerce e T (subst v Ur) s -> P
+        forall s, coerce e T (subst v Ur) s -> P
     | Pair T' u v => 
         forall U s1, typ e U (Srt s1) ->
 	  typ e u U -> 
-	  forall V, typ e v (subst u V) -> T' = (Sum U V) -> coerce e T (Sum U V) s -> P
+	  forall V, typ e v (subst u V) -> T' = (Sum U V) -> 
+        forall s, coerce e T (Sum U V) s -> P
     | Prod A B =>
         forall s1 s2,
-        typ e A (Srt s1) -> typ (A :: e) B (Srt s2) -> s = kind -> coerce e T (Srt s2) s -> P
+        typ e A (Srt s1) -> typ (A :: e) B (Srt s2) ->
+        (T = Srt kind \/ coerce e T (Srt s2) kind) -> P
     | Sum A B =>
         forall s1 s2,
-        typ e A (Srt s1) -> typ (A :: e) B (Srt s2) -> s = kind -> coerce e T (Srt s2) s -> P
+        typ e A (Srt s1) -> typ (A :: e) B (Srt s2) -> 
+        sum_sort A B s1 s2 ->
+        (T = Srt kind \/ coerce e T (Srt s2) kind) -> P
     | Subset A B =>
-        typ e A (Srt set) -> typ (A :: e) B (Srt prop) -> s = kind -> coerce e T (Srt set) s -> P
+        forall s1 s2,
+        s1 = set -> s2 = prop ->
+        typ e A (Srt s1) -> typ (A :: e) B (Srt s2) -> coerce e T (Srt s1) kind -> P
     | Pi1 t =>
         forall U V,
-        typ e t (Sum U V) -> 
-        coerce e T U s -> P
+        typ e t (Sum U V) ->        
+        forall s, coerce e T U s -> P
     | Pi2 t =>
         forall U V,
         typ e t (Sum U V) -> 
-        coerce e T (subst (Pi1 t) V) s -> P
+        forall s, coerce e T (subst (Pi1 t) V) s -> P
     | Let_in t v =>
         forall U, typ e t U -> 
 	forall s1, typ e U (Srt s1) ->
         forall M, typ (U :: e) v M -> 
-        coerce e T (subst t M) s -> P
+        forall s, coerce e T (subst t M) s -> P
     end.
 
-Lemma inv_type_coerce : forall (P : Prop) e t (U V : term) s,
-  inv_type P e t U s -> coerce e U V s -> inv_type P e t V s.
+Lemma unicity_coerce_l : forall e U V s s', e |- U >> V : s -> e |- U : Srt s' -> e |- U >> V : s'.
+Proof.
+  intros.
+  pose (coerce_sort_l _ _ _ _ H).
+  rewrite (unique_sort H0 t).
+  assumption.
+Qed.
+
+Lemma unicity_coerce_r : forall e U V s s', e |- U >> V : s -> e |- V : Srt s' -> e |- U >> V : s'.
+Proof.
+  intros.
+  pose (coerce_sort_r _ _ _ _ H).
+  rewrite (unique_sort H0 t).
+  assumption.
+Qed.
+
+Hint Resolve unicity_coerce_l unicity_coerce_r : coc.
+
+
+Lemma inv_type_coerce : forall (P : Prop) e t (U V : term),
+  inv_type P e t U -> forall s, coerce e U V s -> inv_type P e t V.
 intros P e.
-induction t ; simpl in |- *; intros U V s' H Hco ; intros.
+cut (forall U V W s s', e |- U >> V : s -> e |- V >> W : s' -> e |- U >> W : s') ; intro Htr.
+cut (forall U V W s s', e |- U >> V : s' -> e |- V >> W : s -> e |- U >> W : s') ; intro Htr2.
+induction t ; simpl in |- *; intros U V H s' Hco ; intros.
 destruct (coerce_sort e _ _ s' Hco).
 generalize H ; clear H.
 elim s; auto with coc core arith datatypes; intros ;
-rewrite H2 in H1 ; elim (typ_not_kind _ _ _ H1) ; auto.
+rewrite H2 in H1 ; elim (typ_not_kind H1) ; auto.
 
-apply H with x ; auto with coc core arith datatypes.
-eapply coerce_sort_l with V ; auto with coc core.
-eapply coerce_trans with V ; auto with coc core.
+apply H with x s ; auto with coc core arith datatypes.
+apply Htr with V s' ; auto.
 
-apply H with s1 U0; auto with coc core arith datatypes.
-eapply coerce_trans with V ; auto with coc core.
+apply H with s1 U0 s'; auto with coc core arith datatypes.
+apply Htr2 with V s ; auto.
 
-apply H with Ur V0; auto with coc core arith datatypes.
-eapply coerce_sort_l with V ; auto with coc core.
-eapply coerce_trans with V ; auto with coc core.
+apply H with Ur V0 s; auto with coc core arith datatypes.
+apply Htr with V s' ; auto.
 
-apply H with U0 s1 V0 ; auto with coc core arith datatypes.
-eapply coerce_trans with V ; auto with coc core.
+apply H with U0 s1 V0 s' ; auto with coc core arith datatypes.
+apply Htr2 with V s ; auto.
 
 apply H with s1 s2; auto with coc core arith datatypes.
-eapply coerce_trans with V ; auto with coc core.
+destruct H2.
+rewrite H2 in Hco.
+elim coerce_not_kind_r with e U s' ; auto.
+right.
+apply Htr with V s' ; auto.
 
 apply H with s1 s2; auto with coc core arith datatypes.
-eapply coerce_trans with V ; auto with coc core.
+destruct H3.
+rewrite H3 in Hco.
+elim coerce_not_kind_r with e U s' ; auto.
+right.
+apply Htr with V s' ; auto.
 
-apply H ; auto with coc core arith datatypes.
-eapply coerce_trans with V ; auto with coc core.
+apply H with s1 s2 ; auto with coc core arith datatypes.
+apply Htr with V s' ; auto.
 
-apply H with U0 V0; auto with coc core arith datatypes.
-eapply coerce_trans with V ; auto with coc core.
+apply H with U0 V0 s; auto with coc core arith datatypes.
+apply Htr with V s' ; auto.
 
-apply H with U0 V0; auto with coc core arith datatypes.
-eapply coerce_trans with V ; auto with coc core.
+apply H with U0 V0 s'; auto with coc core arith datatypes.
+apply Htr2 with V s ; auto.
 
-apply H with U0 s1 M; auto with coc core arith datatypes.
-eapply coerce_trans with V ; auto with coc core.
+apply H with U0 s1 M s; auto with coc core arith datatypes.
+apply Htr with V s' ; auto.
+
+intros.
+eapply coerce_trans with V ; auto with coc.
+apply unicity_coerce_l with s ; auto.
+exact (coerce_sort_r _ _ _ _ H).
+
+intros.
+eapply coerce_trans with V ; auto with coc.
+apply unicity_coerce_r with s ; auto.
+exact (coerce_sort_l _ _ _ _ H0).
 Qed.
 
-(*
-Lemma inv_type_sort : forall P e t V s, 
-  e |- V : Srt s -> inv_type P e t V s -> 
-  forall s', e |- V : Srt s' -> inv_type P e t V s'.
+Theorem typ_inversion :
+  forall (P : Prop) e t T, typ e t T -> inv_type P e t T -> P.
 Proof.
-  induction t; simpl ; intros ; auto with coc.
-  apply H0 with x ; auto with coc core arith.
-  *)
+intros.
+pose (type_sorted H).
+rename H into Ht.
+generalize Ht H0 o ; clear H0 o.
+induction 1; simpl in |- *; intros ; 
+auto with coc core arith datatypes.
+
+elim H0; intros.
+induction (wf_sort_lift _ _ _ H H0).
+apply H1 with x x0; auto with coc core arith datatypes.
+rewrite <- H2.
+apply coerce_refl ; auto with coc core.
+
+destruct o ; try discriminate.
+destruct H.
+apply H0 with s1 U x; auto with coc core arith datatypes.
+
+destruct o.
+pose (typ_not_kind Ht0_1).
+pose (subst_to_sort _ H n).
+rewrite e0 in Ht0_2.
+pose (type_no_kind_prod_type Ht0_2).
+simpl in t.
+intuition.
+
+destruct H.
+apply H0 with Ur V x; auto with coc core arith datatypes.
+
+destruct o ; try discriminate.
+destruct H1.
+apply H0 with U s1 V x; auto with coc core arith datatypes.
+
+destruct o.
+apply H0 with s1 s2 ; auto with coc.
+destruct H.
+apply H0 with s1 s2 ; auto with coc.
+right.
+destruct (typ_sort _ _ _ H) ; auto with coc.
+cut (wf e) ; auto with coc.
+apply (typ_wf _ _ _ H).
+
+
+destruct o.
+apply H0 with s1 s2 ; auto with coc.
+destruct H1.
+apply H0 with s1 s2 ; auto with coc.
+right.
+destruct (typ_sort _ _ _ H1) ; auto with coc.
+cut (wf e) ; auto with coc.
+apply (typ_wf _ _ _ H1).
+
+destruct o ; try discriminate.
+destruct H.
+
+apply H0 with set prop; auto with coc core arith datatypes.
+cut (wf e) ; auto with coc.
+apply (typ_wf _ _ _ H).
+
+destruct o.
+pose (sort_of_pi1_range Ht).
+rewrite H in e0.
+simpl in e0.
+destruct (e0 kind (refl_equal (Srt kind))).
+clear e0.
+do 2 destruct H1 ; intuition.
+unfold sum_sort in H4.
+do 2 destruct H4.
+rewrite H4 in H1 ; simpl in H1 ; discriminate.
+discriminate.
+
+destruct H.
+apply H0 with U V x; auto with coc core arith datatypes.
+
+destruct o.
+pose (sort_of_pi2_range Ht).
+rewrite H in e0.
+simpl in e0.
+destruct (e0 kind (refl_equal (Srt kind))).
+clear e0.
+do 2 destruct H1 ; intuition.
+unfold sum_sort in H4.
+do 2 destruct H4.
+destruct (type_range_subst _ _ _ H1).
+simpl ; discriminate.
+rewrite H5 in H6 ; simpl in H6 ; discriminate.
+discriminate.
+
+destruct H.
+apply H0 with U V x; auto with coc core arith datatypes.
+
+pose (coerce_sym _ _ _ _ H).
+apply IHHt0_1 ; auto with coc core arith.
+pose (inv_type_coerce).
+cut (inv_type P e t V).
+intro invt.
+apply (i _ _ _ _ _ invt _ c) ; auto.
+assumption.
+
+pose (coerce_sort_l _ _ _ _ H).
+right ; exists s ; auto.
+Qed.
 
 
 Lemma typ_sort_kind : forall G s s', G |- Srt s : Srt s' -> s' = kind.
@@ -122,117 +262,14 @@ Proof.
   auto.
 Qed.
 
-Theorem typ_inversion_typ :
-  forall (P : Prop) e t T, typ e t T -> forall s, typ e T (Srt s) -> inv_type P e t T s -> P.
-Proof.
-induction 1; simpl in |- *; intros.
-auto with coc core arith datatypes.
 
-auto with coc core arith datatypes.
-
-elim H0; intros.
-apply H2 with x; auto with coc core arith datatypes.
-rewrite H3.
-apply coerce_refl ; auto with coc core.
-rewrite <- H3 ; auto.
-
-apply H3 with s1 U; auto with coc core arith datatypes.
-
-apply H2 with Ur V; auto with coc core arith datatypes.
-
-apply H5 with U s1 V; auto with coc core arith datatypes.
-
-apply H2 with s1 s2; auto with coc core arith datatypes.
-apply (typ_sort_kind H1).
-
-apply H3 with s1 s2; auto with coc core arith datatypes.
-apply (typ_sort_kind H2).
-
-apply H2; auto with coc core arith datatypes.
-apply (typ_sort_kind H1).
-
-apply H1 with U V; auto with coc core arith datatypes.
-
-apply H1 with U V; auto with coc core arith datatypes.
-
-pose (coerce_sym _ _ _ _ H2).
-apply IHtyp1 with s ; auto with coc core arith.
-pose (inv_type_coerce).
-cut (inv_type P e t V s).
-intro invt.
-apply (i _ _ _ _ _ _ invt c).
-pose (unique_sort H0 H3).
-rewrite e0.
-apply H4.
-Qed.
-
-Definition inv_type (P : Prop) e t T s : Prop :=
-  match t with
-    | Srt prop => T = (Srt kind) -> P
-    | Srt set => T = (Srt kind) -> P
-    | Srt kind => True
-    | Ref n => forall x : term, item _ x e n -> 
-       e |- T : Srt s -> e |- T >> (lift (S n) x) : s -> P
-    | Abs A M =>
-        forall s1 (U : term),
-        typ e A (Srt s1) ->
-        typ (A :: e) M U -> coerce e T (Prod A U) s -> P
-    | App u v =>
-        forall Ur V : term,
-        typ e v V -> typ e u (Prod V Ur) -> 
-        typ e T (Srt s) ->
-        coerce e T (subst v Ur) s -> P
-    | Pair T' u v => 
-        forall U s1, typ e U (Srt s1) ->
-	  typ e u U -> 
-	  forall V, typ e v (subst u V) -> T' = (Sum U V) -> coerce e T (Sum U V) s -> P
-    | Prod A B =>
-        forall s1 s2,
-        typ e A (Srt s1) -> typ (A :: e) B (Srt s2) -> s = kind -> coerce e T (Srt s2) s -> P
-    | Sum A B =>
-        forall s1 s2,
-        typ e A (Srt s1) -> typ (A :: e) B (Srt s2) -> s = kind -> coerce e T (Srt s2) s -> P
-    | Subset A B =>
-        typ e A (Srt set) -> typ (A :: e) B (Srt prop) -> s = kind -> coerce e T (Srt set) s -> P
-    | Pi1 t =>
-        forall U V,
-        typ e t (Sum U V) -> 
-        coerce e T U s -> P
-    | Pi2 t =>
-        forall U V,
-        typ e t (Sum U V) -> 
-        coerce e T (subst (Pi1 t) V) s -> P
-    | Let_in t v =>
-        forall U, typ e t U -> 
-	forall s1, typ e U (Srt s1) ->
-        forall M, typ (U :: e) v M -> 
-        coerce e T (subst t M) s -> P
-    end.
-
-
-Theorem typ_inversion :
-  forall (P : Prop) e t T, typ e t T -> forall s, inv_type P e t T s -> P.
-Proof.
-  intros.
-  destruct (type_sorted H).
-  
-
-  rewrite H0.
-  simpl.
-
-  Lemma inv_typ_kind : forall e t, ~ typ e (Srt kind) t.
-red in |- *; intros.
-apply typ_inversion with e (Srt kind) t; simpl in |- *;
- auto with coc core arith datatypes.
-Qed.
-
-  Lemma inv_typ_prop : forall e T, typ e (Srt prop) T -> coerce e T (Srt kind).
+  Lemma inv_typ_prop : forall e T, typ e (Srt prop) T -> T = (Srt kind) .
 intros.
-apply typ_inversion with e (Srt prop) T; simpl in |- *;
+apply typ_inversion with e (Srt prop) T ; simpl in |- *;
  auto with coc core arith datatypes.
 Qed.
 
-  Lemma inv_typ_set : forall e T, typ e (Srt set) T -> coerce e T (Srt kind).
+  Lemma inv_typ_set : forall e T, typ e (Srt set) T -> T = (Srt kind).
 intros.
 apply typ_inversion with e (Srt set) T; simpl in |- *;
  auto with coc core arith datatypes.
@@ -241,103 +278,182 @@ Qed.
   Lemma inv_typ_ref :
    forall (P : Prop) e T n,
    typ e (Ref n) T ->
-   (forall U : term, item _ U e n -> coerce e T (lift (S n) U) -> P) -> P.
+   (forall s, e |- T : Srt s -> forall U : term, item _ U e n -> e |- T >> (lift (S n) U) : s -> P) -> P.
 intros.
 apply typ_inversion with e (Ref n) T; simpl in |- *; intros;
  auto with coc core arith datatypes.
-apply H0 with x; auto with coc core arith datatypes.
+apply H0 with s x; auto with coc core arith datatypes.
+apply (coerce_sort_l _ _ _ _ H2).
 Qed.
 
   Lemma inv_typ_abs :
    forall (P : Prop) e A M (U : term),
    typ e (Abs A M) U ->
-   (forall s1 s2 T,
+   (forall s, e |- U : Srt s ->
+    forall s1 T,
     typ e A (Srt s1) ->
-    typ (A :: e) M T -> typ (A :: e) T (Srt s2) -> coerce e (Prod A T) U -> P) ->
+    typ (A :: e) M T -> 
+    typ (A :: e) T (Srt s) ->
+    e |- (Prod A T) >> U : s -> P) ->
    P.
 intros.
 apply typ_inversion with e (Abs A M) U; simpl in |- *;
  auto with coc core arith datatypes; intros.
-apply H0 with s1 s2 U0; auto with coc core arith datatypes.
+
+pose (coerce_sym _ _ _ _ H3).
+apply H0 with s s1 U0; auto with coc core arith datatypes.
+apply (coerce_sort_l _ _ _ _ H3).
+pose (coerce_sort_r _ _ _ _ H3).
+destruct (generation_prod2 t).
+assumption.
 Qed.
 
-  Lemma inv_typ_app :
-   forall (P : Prop) e u v T,
-   typ e (App u v) T ->
-   (forall V Ur : term,
-    typ e u (Prod V Ur) -> typ e v V -> coerce e T (subst v Ur) -> P) -> P.
+Lemma inv_typ_app :
+ forall (P : Prop) e u v T,
+ typ e (App u v) T ->
+ (forall s, e |- T : Srt s ->
+ forall V Ur : term,
+ typ e u (Prod V Ur) -> typ e v V -> coerce e T (subst v Ur) s -> P) -> P.
 intros.
 apply typ_inversion with e (App u v) T; simpl in |- *;
  auto with coc core arith datatypes; intros.
-apply H0 with V Ur; auto with coc core arith datatypes.
+
+apply H0 with s V Ur; auto with coc core arith datatypes.
+apply (coerce_sort_l _ _ _ _ H3).
 Qed.
 
   Lemma inv_typ_pair :
    forall (P : Prop) e T u v T',
    typ e (Pair T u v) T' ->
-   (forall T U V : term, forall s1 s2,
+   (forall s, e |- T' : Srt s ->
+     forall T U V : term, forall s1,
      typ e U (Srt s1) ->
-     typ e u U -> typ (U :: e) V (Srt s2) -> typ e v (subst u V) ->
-     T = (Sum U V) -> coerce e T' (Sum U V) -> P) -> P.
+     typ e u U -> typ (U :: e) V (Srt s) -> typ e v (subst u V) ->
+     T = (Sum U V) -> coerce e T' (Sum U V) s -> P) -> P.
 intros.
 apply typ_inversion with e (Pair T u v) T'; simpl in |- *;
  auto with coc core arith datatypes; intros.
-apply H0 with T U V s1 s2 ; auto with coc core arith datatypes.
+
+apply H0 with s T U V s1 ; auto with coc core arith datatypes.
+
+apply (coerce_sort_l _ _ _ _ H5).
+pose (coerce_sort_r _ _ _ _ H5).
+destruct (generation_sum2 t).
+intuition.
 Qed.
 
   Lemma inv_typ_prod :
    forall (P : Prop) e T (U s : term),
    typ e (Prod T U) s ->
    (forall s1 s2,
-    typ e T (Srt s1) -> typ (T :: e) U (Srt s2) -> coerce e (Srt s2) s -> P) -> P.
+    typ e T (Srt s1) -> typ (T :: e) U (Srt s2) -> 
+    (s2 = kind \/ coerce e (Srt s2) s kind) -> P) -> P.
 intros.
 apply typ_inversion with e (Prod T U) s; simpl in |- *;
  auto with coc core arith datatypes; intros.
+
 apply H0 with s1 s2; auto with coc core arith datatypes.
+destruct H3.
+left.
+rewrite H3 in H.
+destruct (generation_prod2 H).
+exact (unique_sort H2 H5).
+
+right.
+exact (coerce_sym _ _ _ _ H3).
 Qed.
 
-  Lemma inv_typ_sum :
+Lemma inv_typ_prod2 :
+   forall (P : Prop) e T (U s : term),
+   typ e (Prod T U) s ->
+   (forall s1,
+    typ e T (Srt s1) -> typ (T :: e) U s -> P) -> P.
+intros.
+apply typ_inversion with e (Prod T U) s; simpl in |- *;
+ auto with coc core arith datatypes; intros.
+
+apply H0 with s1; auto with coc core arith datatypes.
+induction H3.
+destruct H3.
+left.
+rewrite H3 in H.
+destruct (generation_prod2 H).
+
+exact (unique_sort H2 H5).
+
+right.
+exact (coerce_sym _ _ _ _ H3).
+Qed.
+
+Lemma inv_typ_sum :
    forall (P : Prop) e T (U s : term),
    typ e (Sum T U) s ->
    (forall s1 s2,
-    typ e T (Srt s1) -> typ (T :: e) U (Srt s2) -> coerce e (Srt s2) s -> P) -> P.
+    typ e T (Srt s1) -> typ (T :: e) U (Srt s2) -> 
+    (s2 = kind \/ coerce e (Srt s2) s kind) -> P) -> P.
 intros.
 apply typ_inversion with e (Sum T U) s; simpl in |- *;
  auto with coc core arith datatypes; intros.
+
 apply H0 with s1 s2; auto with coc core arith datatypes.
+destruct H4.
+left.
+rewrite H4 in H.
+destruct (generation_sum2 H).
+intuition.
+exact (unique_sort H2 H5).
+
+right.
+exact (coerce_sym _ _ _ _ H4).
 Qed.
 
   Lemma inv_typ_subset :
    forall (P : Prop) e T (U s : term),
    typ e (Subset T U) s ->
-   (typ e T (Srt set) -> typ (T :: e) U (Srt prop) -> coerce e (Srt set) s -> P) -> P.
+   (typ e T (Srt set) -> typ (T :: e) U (Srt prop) -> coerce e (Srt set) s kind -> P) -> P.
 intros.
 apply typ_inversion with e (Subset T U) s; simpl in |- *;
  auto with coc core arith datatypes; intros.
+
+rewrite H1 in H3.
+rewrite H2 in H4.
+apply H0 ; auto.
+rewrite H1 in H5.
+exact (coerce_sym _ _ _ _ H5).
 Qed.
 
 Lemma inv_typ_pi1 : 
   forall (P : Prop) e t T,
    typ e (Pi1 t) T ->
-   (forall U V, typ e t (Sum U V) ->  coerce e U T -> P) -> P.
+   (forall s, typ e T (Srt s) ->
+   forall U V, typ e t (Sum U V) -> 
+   coerce e U T s -> P) -> P.
 Proof.
 intros.
 apply typ_inversion with e (Pi1 t) T; simpl in |- *;
  auto with coc core arith datatypes; intros.
-apply H0 with U V ; auto with coc.
+
+apply H0 with s U V ; auto with coc.
+exact (coerce_sort_l _ _ _ _ H2).
+
+apply coerce_sym ; auto.
 Qed.
 
 Lemma inv_typ_pi2 : 
   forall (P : Prop) e t T,
    typ e (Pi2 t) T ->
-   (forall U V, typ e t (Sum U V) ->  coerce e (subst (Pi1 t) V) T -> P) -> P.
+   (forall s, typ e T (Srt s) -> forall U V, typ e t (Sum U V) ->  coerce e (subst (Pi1 t) V) T s -> P) -> P.
 Proof.
 intros.
 apply typ_inversion with e (Pi2 t) T; simpl in |- *;
  auto with coc core arith datatypes; intros.
-apply H0 with U V ; auto with coc.
-Qed.
 
+apply H0 with s U V ; auto with coc.
+exact (coerce_sort_l _ _ _ _ H2).
+
+apply coerce_sym ; auto.
+Qed.
+(
 Lemma inv_typ_let_in : 
   forall (P : Prop) e v t T,
    typ e (Let_in v t) T ->
@@ -353,13 +469,16 @@ apply typ_inversion with e (Let_in v t) T; simpl in |- *;
 apply (H0 U H1 s1 H2 M H3 s2 H4) ; auto with coc.
 Qed.
 
+*)
+
 
   Lemma typ_mem_kind : forall e t T, mem_sort kind t -> ~ typ e t T.
-red in |- *; intros.
+red in |- * ; intros.
+
 apply typ_inversion with e t T; auto with coc core arith datatypes.
 generalize e T.
 clear H0.
-elim H; simpl in |- *; auto with coc core arith datatypes; intros.
+elim H; simpl in |- * ; auto with coc core arith datatypes; intros.
 apply typ_inversion with e0 u (Srt s1); auto with coc core arith datatypes.
 
 apply typ_inversion with (u :: e0) v (Srt s2);
@@ -367,16 +486,19 @@ apply typ_inversion with (u :: e0) v (Srt s2);
 
 apply typ_inversion with e0 u (Srt s1); auto with coc core arith datatypes.
 
+
+
 apply typ_inversion with (u :: e0) v U; auto with coc core arith datatypes.
 
 apply typ_inversion with e0 u (Prod V Ur); auto with coc core arith datatypes.
 
 apply typ_inversion with e0 v V; auto with coc core arith datatypes.
 
-rewrite H6 in H0.
-rewrite H6 in H1.
-simpl in H1.
-apply H1 with e0 (Srt s2) s1 s2 ;  auto with coc core arith datatypes.
+pose (coerce_sort_r _ _ _ _ H6).
+rewrite <- H5 in t0.
+
+apply typ_inversion with e0 T0 (Srt s); auto with coc core arith datatypes.
+
 apply typ_inversion with e0 u U; auto with coc core arith datatypes.
 apply typ_inversion with e0 v (subst u V); auto with coc core arith datatypes.
 
@@ -384,8 +506,10 @@ apply typ_inversion with e0 u (Srt s1); auto with coc core arith datatypes.
 
 apply typ_inversion with (u :: e0) v (Srt s2); auto with coc core arith datatypes.
 
+rewrite H2 in H4.
 apply typ_inversion with e0 u (Srt set); auto with coc core arith datatypes.
 
+rewrite H3 in H5.
 apply typ_inversion with (u :: e0) v (Srt prop); auto with coc core arith datatypes.
 
 apply typ_inversion with e0 u (Sum U V); auto with coc core arith datatypes.
@@ -397,8 +521,7 @@ apply typ_inversion with e0 u U; auto with coc core arith datatypes.
 apply typ_inversion with (U :: e0) v M; auto with coc core arith datatypes.
 Qed.
 
-
-  Lemma inv_typ_conv_kind : forall e t T, conv t (Srt kind) -> ~ typ e t T.
+Lemma inv_typ_conv_kind : forall e t T, conv t (Srt kind) -> ~ typ e t T.
 intros.
 apply typ_mem_kind.
 apply red_sort_mem.
@@ -409,13 +532,16 @@ red in |- *; red in |- *; intros.
 inversion_clear H2.
 Qed.
 
-Lemma type_pair_unique : forall e t T, typ e t T -> forall U V u v, t = (Pair (Sum U V) u v) ->
-   coerce e T (Sum U V).
+(*Lemma type_pair_unique : forall e t T, e |- t : T -> 
+   forall U V u v, t = (Pair (Sum U V) u v) ->
+   exists s, e |- T >> (Sum U V) : s.
 Proof.
-intros ; induction H ; try discriminate.
-injection H0 ; intros.
-rewrite H6 ; rewrite H7.
-apply refl_coerce.
+induction 1 ; intros ;  try discriminate.
+injection H4 ; intros.
+exists s2.
+rewrite H7 ; rewrite H8.
+apply coerce_refl ; auto with coc.
+apply type_sum with s1.
 pose (IHtyp1 H0).
 apply coerce_trans with U0; auto with coc core arith datatypes.
 Qed.
@@ -436,3 +562,4 @@ exists x ; exists x0.
 split ; auto with coc.
 apply coerce_trans with U; auto with coc core arith datatypes.
 Qed.
+*)
